Add: +2

theories/Main.v
@@ -956,14 +956,33 @@ Proof.
     exact (inv (conc_1_p (p x))).
 Defined.
 
+Definition ap1@{i j | }
+  {A : Type@{i}} {B : Type@{j}} (f : A -> B) {x x' : A} (p : Path@{i} x x')
+  : Path@{j} (f x) (f x').
+Proof.
+  refine (match p with idpath => _ end).
+  exact idpath.
+Defined.
+
 Definition ap2@{i j k | }
   {A : Type@{i}} {B : Type@{j}} {C : Type@{k}} (f : A -> B -> C)
   {x x' : A} (p : Path@{i} x x') {y y' : B} (q : Path@{j} y y')
   : Path@{k} (f x y) (f x' y').
 Proof.
   refine (match p with idpath => _ end).
-  refine (ap (f x) _).
-  exact q.
+  exact (ap1 (f x) q).
+Defined.
+
+Definition ap3@{i j k l | }
+  {A : Type@{i}} {B : Type@{j}} {C : Type@{k}} {D : Type@{l}}
+  (f : A -> B -> C -> D)
+  {x x' : A} (p : Path@{i} x x')
+  {y y' : B} (q : Path@{j} y y')
+  {z z' : C} (r : Path@{k} z z')
+  : Path@{l} (f x y z) (f x' y' z').
+Proof.
+  refine (match p with idpath => _ end).
+  refine (ap2 (f x) q r).
 Defined.
 
 (** Path_conc_conc_r_ap_f_q_conc_p_y_s_conc_conc_r_p_x_conc_ap_g_q_s です。 *)
